Converted 5 files to use the freezer. Single-core compilation time now 38mins (from 61mins)

tweetnacl20140427/verif_fcore_epilogue_htrue.v
@@ -21,7 +21,7 @@ Definition HTrue_inv1 l i ys xs : Prop :=
                                       Znth j l Vundef = Vint (Int.add yj xj)) 
                 /\ (i<=j ->  Znth j l Vundef = Vint xj).
 
-Lemma HTrue_loop1 Espec: forall t y x w nonce out c k h data OUT xs ys,
+Lemma HTrue_loop1 Espec: forall (FR:mpred) t y x w nonce out c k h xs ys,
 @semax CompSpecs Espec
   (initialized_list [_i] (func_tycontext f_core SalsaVarSpecs SalsaFunSpecs))
   (PROP  ()
@@ -29,10 +29,8 @@ Lemma HTrue_loop1 Espec: forall t y x w nonce out c k h data OUT xs ys,
    lvar _y (tarray tuint 16) y; lvar _x (tarray tuint 16) x;
    lvar _w (tarray tuint 16) w; temp _in nonce; temp _out out; temp _c c;
    temp _k k; temp _h (Vint (Int.repr h)))
-   SEP  (data_at Tsh (tarray tuint 16) (map Vint xs) x;
-   data_at Tsh (tarray tuint 16) (map Vint ys) y;
-   data_at_ Tsh (tarray tuint 4) t; data_at_ Tsh (tarray tuint 16) w;
-   CoreInSEP data (nonce, c, k); data_at Tsh (tarray tuchar 64) OUT out))
+   SEP  (FR; data_at Tsh (tarray tuint 16) (map Vint xs) x;
+         data_at Tsh (tarray tuint 16) (map Vint ys) y))
   (Sfor (Sset _i (Econst_int (Int.repr 0) tint))
      (Ebinop Olt (Etempvar _i tint) (Econst_int (Int.repr 16) tint) tint)
      (Ssequence
@@ -59,14 +57,12 @@ Lemma HTrue_loop1 Espec: forall t y x w nonce out c k h data OUT xs ys,
              lvar _y (tarray tuint 16) y; lvar _x (tarray tuint 16) x;
              lvar _w (tarray tuint 16) w; temp _in nonce; temp _out out;
              temp _c c; temp _k k; temp _h (Vint (Int.repr h)))
-     SEP (data_at Tsh (tarray tuint 16) l x;
-          data_at Tsh (tarray tuint 16) (map Vint ys) y;
-          data_at_ Tsh (tarray tuint 4) t; data_at_ Tsh (tarray tuint 16) w;
-          CoreInSEP data (nonce, c, k); data_at Tsh (tarray tuchar 64) OUT out))).
+     SEP (FR; data_at Tsh (tarray tuint 16) l x;
+          data_at Tsh (tarray tuint 16) (map Vint ys) y))).
 Proof. 
   intros. abbreviate_semax.
   Time assert_PROP (Zlength (map Vint xs) = 16 /\ Zlength (map Vint ys) = 16) 
-     as XLYL by entailer!. (*2.6*)
+     as XLYL by entailer!. (*2 versus 2.6*)
   destruct XLYL as [XL YL].
   Time forward_for_simple_bound 16 (EX i:Z, 
    (PROP  ()
@@ -74,14 +70,12 @@ Proof.
    lvar _y (tarray tuint 16) y; lvar _x (tarray tuint 16) x;
    lvar _w (tarray tuint 16) w; temp _in nonce; temp _out out; temp _c c;
    temp _k k; temp _h (Vint (Int.repr h)))
-   SEP  (EX l:_, !!HTrue_inv1 l i (map Vint ys) (map Vint xs)
+   SEP  (FR;
+         EX l:_, !!HTrue_inv1 l i (map Vint ys) (map Vint xs)
               && data_at Tsh (tarray tuint 16) l x;
-   data_at Tsh (tarray tuint 16) (map Vint ys) y;
-   data_at_ Tsh (tarray tuint 4) t; data_at_ Tsh (tarray tuint 16) w;
-   CoreInSEP data (nonce, c, k);
-   data_at Tsh (tarray tuchar 64) OUT out))). (*3.3*)
+         data_at Tsh (tarray tuint 16) (map Vint ys) y))). (*1.2 versus 3.3*)
   { Exists (map Vint xs).
-    Time entailer!. (*3.9*)
+    Time entailer!. (*3.3 versus 3.9*)
     split. assumption.
     exists xs; split; trivial.
     intros. 
@@ -93,13 +87,13 @@ Proof.
     destruct XLIST as [xints [INTS J]]. subst xlist.
     destruct (J _ I) as [xi [Xi [_ HXi]]].
     destruct (Znth_mapVint ys i Vundef) as [yi Yi]. rewrite Zlength_map in YL; omega.
-    Time forward; rewrite Yi. (*7.2*)
-    Time solve[entailer!]. (*2.7*)
-    Time forward; rewrite HXi by omega. (*12.3*)
-    Time solve[entailer!]. (*3.6*) 
-    Time forward. (*12.1*) 
+    Time forward; rewrite Yi. (*6 versus 7.2*)
+    Time solve[entailer!]. (*2 versus 2.7*)
+    Time forward; rewrite HXi by omega. (*5.7 versus 7.4*)
+    Time solve[entailer!]. (*1.6 versus 2.6*) 
+    Time forward. (*5.9 versus 7.4*) 
     Exists (upd_Znth i (map Vint xints) (Vint (Int.add yi xi))).
-    Time entailer!. (*6.8*) (*
+    Time entailer!. (*3.9 versus 4.6*) (*
     rewrite Yi in H1. symmetry in H1; inv H1. rewrite Yi, HXi; simpl. 2: omega. 
     apply (exp_right (upd_Znth i (map Vint xints) (Vint (Int.add yi xi)))); entailer.
     apply prop_right.*)
@@ -123,9 +117,9 @@ Proof.
             simpl in *; omega.
             simpl in *; omega.
             omega. }
-Time entailer!. (*9.8*)
+Time entailer!. (*4.5 versus 9.8*)
 Exists l. Time entailer!. (*3.2*) 
-Time Qed. (*24*)
+Time Qed. (*19.3 versus 24*)
 
 (* Fragment:
        FOR(i,4) {
@@ -142,7 +136,7 @@ Fixpoint hPosLoop2 (n:nat) (sumlist: list int) (C Nonce: SixteenByte): list int 
                 upd_Znth (6+j) (upd_Znth (5*j) s five) six
        end.
 
-Lemma HTrue_loop2 Espec: forall t y x w nonce out c k h OUT ys intsums Nonce C K,
+Lemma HTrue_loop2 Espec: forall (FR:mpred) t y x w nonce out c k h (*OUT ys*) intsums Nonce C K,
 @semax CompSpecs Espec 
   (initialized_list [_i] (func_tycontext f_core SalsaVarSpecs SalsaFunSpecs))
   (PROP  ()
@@ -150,11 +144,8 @@ Lemma HTrue_loop2 Espec: forall t y x w nonce out c k h OUT ys intsums Nonce C K
      lvar _y (tarray tuint 16) y; lvar _x (tarray tuint 16) x;
      lvar _w (tarray tuint 16) w; temp _in nonce; temp _out out; temp _c c;
      temp _k k; temp _h (Vint (Int.repr h)))
-   SEP  (data_at Tsh (tarray tuint 16) (map Vint intsums) x;
-     data_at Tsh (tarray tuint 16) (map Vint ys) y;
-     data_at_ Tsh (tarray tuint 4) t; data_at_ Tsh (tarray tuint 16) w;
-     CoreInSEP(Nonce, C, K) (nonce, c, k);
-     data_at Tsh (tarray tuchar 64) OUT out))
+   SEP  (FR; CoreInSEP(Nonce, C, K) (nonce, c, k);
+         data_at Tsh (tarray tuint 16) (map Vint intsums) x))
    (Ssequence (Sset _i (Econst_int (Int.repr 0) tint))
               (Sloop
                 (Ssequence
@@ -224,16 +215,13 @@ Lemma HTrue_loop2 Espec: forall t y x w nonce out c k h OUT ys intsums Nonce C K
                     (Econst_int (Int.repr 1) tint) tint))))
   (normal_ret_assert (PROP  ()
  LOCAL  (temp _i (Vint (Int.repr 4)); lvar _t (tarray tuint 4) t;
- lvar _y (tarray tuint 16) y; lvar _x (tarray tuint 16) x;
- lvar _w (tarray tuint 16) w; temp _in nonce; temp _out out; temp _c c;
- temp _k k; temp _h (Vint (Int.repr h)))
- SEP  (SByte Nonce nonce; SByte C c; ThirtyTwoByte K k;
- data_at Tsh (tarray tuint 16) (map Vint (hPosLoop2 4 intsums C Nonce)) x;
- data_at Tsh (tarray tuint 16) (map Vint ys) y;
- data_at_ Tsh (tarray tuint 4) t; data_at_ Tsh (tarray tuint 16) w;
- data_at Tsh (tarray tuchar 64) OUT out))).
+         lvar _y (tarray tuint 16) y; lvar _x (tarray tuint 16) x;
+         lvar _w (tarray tuint 16) w; temp _in nonce; temp _out out; temp _c c;
+         temp _k k; temp _h (Vint (Int.repr h)))
+ SEP  (FR; SByte Nonce nonce; SByte C c; ThirtyTwoByte K k;
+        data_at Tsh (tarray tuint 16) (map Vint (hPosLoop2 4 intsums C Nonce)) x))).
 Proof. intros. abbreviate_semax. unfold CoreInSEP. 
-  Time assert_PROP (Zlength (map Vint intsums) = 16) as SL by entailer!. (*2.7*)
+  Time assert_PROP (Zlength (map Vint intsums) = 16) as SL by entailer!. (*0.9 versus 2.7*)
   rewrite Zlength_map in SL. 
   Time forward_for_simple_bound 4 (EX i:Z, 
   (PROP  ()
@@ -242,24 +230,21 @@ Proof. intros. abbreviate_semax. unfold CoreInSEP.
    lvar _y (tarray tuint 16) y; lvar _x (tarray tuint 16) x;
    lvar _w (tarray tuint 16) w; temp _in nonce; temp _out out; temp _c c;
    temp _k k; temp _h (Vint (Int.repr h)))
-   SEP  (SByte Nonce nonce; SByte C c; ThirtyTwoByte K k;
-   data_at Tsh (tarray tuint 16) (map Vint (hPosLoop2 (Z.to_nat i) intsums C Nonce)) x;
-   data_at Tsh (tarray tuint 16) (map Vint ys) y;
-   data_at_ Tsh (tarray tuint 4) t; data_at_ Tsh (tarray tuint 16) w;
-   data_at Tsh (tarray tuchar 64) OUT out))). (*3.2*)
-    Time solve[entailer!]. (*3.4*)
+   SEP  (FR; SByte Nonce nonce; SByte C c; ThirtyTwoByte K k;
+   data_at Tsh (tarray tuint 16) (map Vint (hPosLoop2 (Z.to_nat i) intsums C Nonce)) x))). (*1.2 versus 3.2*)
+    Time solve[entailer!]. (*1.6 versus 4.4*)
     { rename H into I.
       unfold SByte at 2.
-      Time assert_PROP (isptr c) as Pc by entailer!. (*4.1*)
+      Time assert_PROP (isptr c) as Pc by entailer!. (*3.2 versus 4.1*)
       apply isptrD in Pc; destruct Pc as [cb [coff HC]]. rewrite HC in *.
       Opaque Zmult. Opaque Z.add. 
 
-      Time forward. (*4.2*)
+      Time forward. (*1.9 versus 4.2*)
       assert (C16:= SixteenByte2ValList_Zlength C).
       remember (SplitSelect16Q C i) as FB; destruct FB as (Front, BACK).
       specialize (Select_SplitSelect16Q C i _ _ HeqFB); intros SSS.
       Time assert_PROP (field_compatible (Tarray tuchar 16 noattr) [] (Vptr cb coff))
-        as FC by entailer!. (*4.3*)
+        as FC by entailer!. (*1.8 versus 4.3*)
       destruct (Select_SplitSelect16Q_Zlength _ _ _ _ HeqFB I) as[FL BL].
 
  (* An alternative to Select_Unselect_Tarray_at is to use
@@ -277,10 +262,11 @@ Proof. intros. abbreviate_semax. unfold CoreInSEP.
       2: rewrite <- SSS, <- C16; cbv; trivial.
   unfold Select_at. repeat rewrite QuadChunk2ValList_ZLength. rewrite Z.mul_1_r, FL.
        simpl. rewrite app_nil_r. simpl. 
-    Time normalize. (*1.4*)
+    Time normalize. (*1.1 versus 1.4*)
       
     Time forward_call ((Vptr cb (Int.add coff (Int.repr (4 * i)))),
-                      Select16Q C i). (*11.1*)
+                      Select16Q C i). (*4.8 versus 10.3*)
+ 
       Intros pat; subst pat.
       assert (PL2length: forall n, (0<=n<4)%nat -> Zlength (hPosLoop2 n intsums C Nonce) = 16).
         clear - SL.
@@ -293,17 +279,17 @@ Proof. intros. abbreviate_semax. unfold CoreInSEP.
         
       destruct (Znth_mapVint (hPosLoop2 (Z.to_nat i) intsums C Nonce) (5*i) Vundef) as [vj Vj].
       rewrite PL2Zlength; omega. 
-      Time forward; rewrite Vj. (*10.9*)
-      Time solve[entailer!]. (*3.6*)
+      Time forward; rewrite Vj. (*5.4 versus 10.9*)
+      Time solve[entailer!]. (*1.4 versus 3.6*)
 
-      Time forward. (*10.3*)
+      Time forward. (*4.9 versus 10.3*)
 
       unfold SByte.
       Time assert_PROP (isptr nonce /\ field_compatible (Tarray tuchar 16 noattr) [] nonce)
-        as PnonceFCN by entailer!. (*4.9*)
+        as PnonceFCN by entailer!. (*1.9 versus 4.9*)
       destruct PnonceFCN as [Pnonce FCN]. 
       apply isptrD in Pnonce; destruct Pnonce as [nb [noff NC]]; rewrite NC in *.
-      Time forward. (*5*)
+      Time forward. (*2.4 versus 5*)
 
       assert (N16:= SixteenByte2ValList_Zlength Nonce).
       remember (SplitSelect16Q Nonce i) as FBN; destruct FBN as (FrontN, BACKN).
@@ -316,23 +302,24 @@ Proof. intros. abbreviate_semax. unfold CoreInSEP.
       2: rewrite <- NNN, <- N16; cbv; trivial.
       unfold Select_at. repeat rewrite QuadChunk2ValList_ZLength. rewrite Zmult_1_r, FN.
       simpl. rewrite app_nil_r. simpl. 
-      Time normalize. (*1.7*) (*rewrite Vj.*)
+      Time normalize. (*1.3 versus 1.7*) (*rewrite Vj.*)
 
       Time forward_call (Vptr nb (Int.add noff (Int.repr (4 * i))),
-                     Select16Q Nonce i). (*15.3*)
+                     Select16Q Nonce i). (*6.6 versus 14.8*)
+
      Intros pat; subst pat. simpl. 
      destruct (Znth_mapVint (hPosLoop2 (Z.to_nat i) intsums C Nonce) (6+i) Vundef) as [uj Uj].
       rewrite PL2Zlength; omega.  
-     Time forward; rewrite upd_Znth_diff; try (rewrite Zlength_map, PL2Zlength; simpl; omega). (*13*)
-     { Time entailer!. (*4.6*)
+     Time forward; rewrite upd_Znth_diff; try (rewrite Zlength_map, PL2Zlength; simpl; omega). (*7.2 versus 13*)
+     { Time entailer!. (*2 versus 4.6*)
        rewrite ZtoNat_Zlength in Uj, PL2Zlength; rewrite Uj.
        simpl; trivial. }
      { omega. } 
-     Time forward. (*12.9 SLOW; was 8*)
+     Time forward. (*5.6 versus 12.9*)
 (*Issue: substitution in entailer/entailer! is a bit too eager here. Without the following assert (FLN: ...) ... destruct FLN,
   the two hypotheses are simply combined to Zlength Front = Zlength FrontN by entailer (and again by the inv H0) *)
      assert (FLN: Zlength Front = i /\ Zlength FrontN = i). split; assumption. clear FL FN.
-     Time entailer!. (*11.6*)
+     Time entailer!. (*6.2 versus 11.6*)
      rewrite Uj in H0. symmetry in H0; inv H0.
      destruct FLN as [FL FLN].
 
@@ -407,8 +394,8 @@ Proof. intros. abbreviate_semax. unfold CoreInSEP.
        rewrite <- UJeq, Zlength_map. reflexivity. apply I.
     +  omega. 
    } 
-  Time entailer!. (*13.3*)
-Time Qed. (*86*)
+  Time entailer!. (*6.6 versus 13.3*)
+Time Qed. (*53 versus 86*)
 
 Definition UpdateOut (l: list val) (i:Z) (xi:int) :=
          (sublist 0 i l) ++ QuadByte2ValList (littleendian_invert xi) ++ sublist (i+4) (Zlength l) l.
@@ -443,7 +430,7 @@ Lemma hposLoop3_length xlist old: forall n, (16+4*Z.of_nat n<Zlength old) ->
     simpl. rewrite IHn. omega. omega. 
   Qed.
 
-Lemma HTrue_loop3 Espec t y x w nonce out c k h OUT xs ys Nonce C K:
+Lemma HTrue_loop3 Espec (FR:mpred) t y x w nonce out c k h OUT xs (*ys Nonce C K*):
 @semax CompSpecs Espec 
   (initialized_list [_i] (func_tycontext f_core SalsaVarSpecs SalsaFunSpecs))
   (PROP  ()
@@ -451,12 +438,8 @@ Lemma HTrue_loop3 Espec t y x w nonce out c k h OUT xs ys Nonce C K:
    lvar _y (tarray tuint 16) y; lvar _x (tarray tuint 16) x;
    lvar _w (tarray tuint 16) w; temp _in nonce; temp _out out; temp _c c;
    temp _k k; temp _h (Vint (Int.repr h)))
-   SEP  (SByte Nonce nonce; SByte C c;
-   ThirtyTwoByte K k;
-   data_at Tsh (tarray tuint 16) (map Vint xs) x;
-   data_at Tsh (tarray tuint 16) (map Vint ys) y;
-   data_at_ Tsh (tarray tuint 4) t; data_at_ Tsh (tarray tuint 16) w;
-   data_at Tsh (tarray tuchar 64) OUT out))
+   SEP  (FR; data_at Tsh (tarray tuchar 64) OUT out;
+         data_at Tsh (tarray tuint 16) (map Vint xs) x))
   (Sfor (Sset _i (Econst_int (Int.repr 0) tint))
      (Ebinop Olt (Etempvar _i tint) (Econst_int (Int.repr 4) tint) tint)
      (Ssequence
@@ -502,25 +485,19 @@ Lemma HTrue_loop3 Espec t y x w nonce out c k h OUT xs ys Nonce C K:
           lvar _y (tarray tuint 16) y; lvar _x (tarray tuint 16) x;
           lvar _w (tarray tuint 16) w; temp _in nonce; temp _out out; temp _c c;
           temp _k k; temp _h (Vint (Int.repr h)))
-  SEP (SByte Nonce nonce; SByte C c; ThirtyTwoByte K k;
-       data_at Tsh (tarray tuint 16) (map Vint xs) x;
-       data_at Tsh (tarray tuint 16) (map Vint ys) y;
-       data_at_ Tsh (tarray tuint 4) t; data_at_ Tsh (tarray tuint 16) w;
+  SEP (FR; data_at Tsh (tarray tuint 16) (map Vint xs) x;
        data_at Tsh (tarray tuchar 64) (hPosLoop3 4 xs OUT) out))).
 Proof. intros. abbreviate_semax.
- Time assert_PROP (Zlength (map Vint xs) = 16 /\ Zlength OUT = 64) as XX by entailer!. (*3.5*)
+ Time assert_PROP (Zlength (map Vint xs) = 16 /\ Zlength OUT = 64) as XX by entailer!. (*1.6 versus 3.5*)
  rewrite Zlength_map in XX. destruct XX as [ZL_X OL].
  Time forward_for_simple_bound 4 (EX i:Z, 
   (PROP  ()
    LOCAL  (lvar _t (tarray tuint 4) t; lvar _y (tarray tuint 16) y;
    lvar _x (tarray tuint 16) x; lvar _w (tarray tuint 16) w; temp _in nonce;
    temp _out out; temp _c c; temp _k k; temp _h (Vint (Int.repr h)))
-   SEP  (SByte Nonce nonce; SByte C c; ThirtyTwoByte K k;
-   data_at Tsh (tarray tuint 16) (map Vint xs) x;
-   data_at Tsh (tarray tuint 16) (map Vint ys) y;
-   data_at_ Tsh (tarray tuint 4) t; data_at_ Tsh (tarray tuint 16) w;
-   data_at Tsh (tarray tuchar 64) (hPosLoop3 (Z.to_nat i) xs OUT) out))). (*3.4*)
-    Time entailer!. (*6*)
+   SEP  (FR; data_at Tsh (tarray tuint 16) (map Vint xs) x;
+         data_at Tsh (tarray tuchar 64) (hPosLoop3 (Z.to_nat i) xs OUT) out))). (*1.6 versus 3.4*)
+    Time entailer!. (*2 versus 6*)
   { rename H into I. 
 
     assert (P3_Zlength: Zlength (hPosLoop3 (Z.to_nat i) xs OUT) = 64).
@@ -530,23 +507,24 @@ Proof. intros. abbreviate_semax.
     remember (hPosLoop3 (Z.to_nat i) xs OUT) as ll. (*clear Heqll.*)
       
     destruct (Znth_mapVint xs (5 * i) Vundef) as [xi Xi]. omega.
-    Time forward; rewrite Xi. (*8.8*)
-    Time solve[entailer!]. (*3.1*)
+    Time forward; rewrite Xi. (*4.8 versus 8.8*)
+    Time solve[entailer!]. (*1.5 versus 3.21*)
     Time assert_PROP (isptr out /\ field_compatible (Tarray tuchar 64 noattr) [] out)
-          as Pout_FCO by entailer!. (*3.6*)
+          as Pout_FCO by entailer!. (*1.8 versus 3.6*)
     destruct Pout_FCO as [Pout FCO].
     apply isptrD in Pout; destruct Pout as [ob [ooff OC]]; rewrite OC in *.
-    Time forward. (*4*)
+    Time forward. (*1.9 versus 4*)
     rewrite <- P3_Zlength.
     rewrite (split3_data_at_Tarray_tuchar Tsh (Zlength ll) (4 *i) (4+4*i)); try rewrite P3_Zlength; trivial; try omega. 
     rewrite field_address0_offset by auto with field_compatible.
     rewrite field_address0_offset by auto with field_compatible.
-    unfold offset_val; simpl.   
-    Time normalize. (*5*)
+    unfold offset_val; simpl.
+    Time normalize. (*4.1 versus 5*)
 
-    Time forward_call (offset_val (Int.repr (4 * i)) (Vptr ob ooff), xi). (*8.2*)
+    Time forward_call (offset_val (Int.repr (4 * i)) (Vptr ob ooff), xi). (*3.6 versus 8.2*)
+
     { Exists (sublist (4 * i) (4 + 4 * i) ll). unfold offset_val; simpl.
-      autorewrite with sublist. Time entailer!. (*10.7*) }
+      autorewrite with sublist. Time entailer!. (*3.7 versus 9.3*) }
     simpl. Opaque mult.
     assert (Upd_ll_Zlength: Zlength (UpdateOut ll (4 * i) xi) = 64).
       rewrite UpdateOut_Zlength; trivial. omega. omega.
@@ -559,12 +537,9 @@ Proof. intros. abbreviate_semax.
    temp _out (Vptr ob ooff); temp _c c; temp _k k;
    temp _h (Vint (Int.repr h)))
    SEP 
-   (data_at Tsh (tarray tuchar 64) (UpdateOut ll (4*i) xi) (Vptr ob ooff);
-   SByte Nonce nonce; SByte C c; ThirtyTwoByte K k;
-   data_at Tsh (tarray tuint 16) (map Vint xs) x;
-   data_at Tsh (tarray tuint 16) (map Vint ys) y;
-   data_at_ Tsh (tarray tuint 4) t; data_at_ Tsh (tarray tuint 16) w))).
-    { clear Heqll. Opaque Zminus. Time entailer!. (*7.5*) unfold QByte.
+   (FR; data_at Tsh (tarray tuchar 64) (UpdateOut ll (4*i) xi) (Vptr ob ooff);
+   data_at Tsh (tarray tuint 16) (map Vint xs) x))).
+    { clear Heqll. Opaque Zminus. Time entailer!. (*5.6 versus 7.5*) unfold QByte.
       rewrite <- Upd_ll_Zlength. unfold tarray. 
       erewrite (split3_data_at_Tarray_tuchar Tsh _ (4 * i) (4+4 * i) (UpdateOut ll (4 * i) _id0)); try rewrite UpdateOut_Zlength, P3_Zlength; try omega.
       rewrite field_address0_offset by auto with field_compatible.
@@ -579,25 +554,25 @@ Proof. intros. abbreviate_semax.
       autorewrite with sublist. rewrite Zplus_comm, AR. trivial. }
  
     destruct (Znth_mapVint xs (6+i) Vundef) as [zi Zi]. omega.
-    Time forward; rewrite Zi. (*11.1*)
-    Time solve[entailer!]. (*3.2*)
-    Time forward. (*4.5*) 
+    Time forward; rewrite Zi. (*6 versus 11.1*)
+    Time solve[entailer!]. (*1.7 versus 3.2*)
+    Time forward. (*2.2 versus 4.5*) 
     erewrite (split3_data_at_Tarray_tuchar Tsh 64 (16 + 4 *i) (4+16 + 4 *i)); trivial; try omega.
     rewrite field_address0_offset by auto with field_compatible.
     rewrite field_address0_offset by auto with field_compatible.
     unfold offset_val; simpl.
     autorewrite with sublist. repeat rewrite Z.mul_1_l. 
 
-    Time forward_call (Vptr ob (Int.add ooff (Int.repr (16 + 4 * i))), zi). (*11.2*)
+    Time forward_call (Vptr ob (Int.add ooff (Int.repr (16 + 4 * i))), zi). (*4.8 versus 11.2*)
     { Exists (sublist (16 + 4 * i) (4 + (16 + 4 * i)) (UpdateOut ll (4 * i) xi)).
       autorewrite with sublist. rewrite Z.add_assoc. 
-      Time entailer!. (*13.5*) }
+      Time entailer!. (*5.1 versus 13.5*) }
 
-    Time entailer!. (*11.5*)
+    Time entailer!. (*8.1 versus 11.5*)
     assert (AA:  Z.to_nat (i + 1) = S (Z.to_nat i)).
       rewrite (Z.add_comm _ 1), Z2Nat.inj_add. simpl. apply NPeano.Nat.add_1_l. omega. omega.
     rewrite AA. simpl. 
-    clear H10 H13 TC TC0 TC1 TC2 TC3 H7.
+    clear H6 H9 TC TC0 TC1 TC2 TC3(* H7*).
     remember (hPosLoop3 (Z.to_nat i) xs OUT) as ll; clear Heqll.
     assert (XXi: xi = Znth (5 * i) xs Int.zero).
       rewrite Znth_map' with (d':=Int.zero) in Xi; try omega. clear -Xi. inv Xi. trivial.
@@ -614,12 +589,12 @@ Proof. intros. abbreviate_semax.
       unfold offset_val. Opaque QuadByte2ValList.  simpl. repeat rewrite Z.mul_1_l.
       Transparent QuadByte2ValList. Transparent Zminus.
       unfold UpdateOut. 
-      autorewrite with sublist. Time cancel. (*1.1*)
+      autorewrite with sublist. Time cancel. (*0.6*)
       rewrite sublist_app2; autorewrite with sublist; try omega.
       rewrite sublist_app2; try rewrite <- QuadByteValList_ZLength; try omega.
       autorewrite with sublist. rewrite Zplus_comm. apply derives_refl'. f_equal. f_equal; omega. }
-  Time entailer!. (*12.8*)
-Time Qed. (*110*)
+  Time entailer!. (*7.9 versus 12.8*) (*With temp _i (Vint (Int.repr 4)) in LOCAL of HTruePostCondL apply derives_refl.*)
+Time Qed. (*62 versus 110*)
 
 Lemma hposLoop2_Zlength16 C N l (L:Zlength l = 16): forall n, 
       5 * Z.of_nat n < 16-> 6+ Z.of_nat n < 16 -> Zlength (hPosLoop2 (S n) l C N) = 16.
@@ -633,7 +608,7 @@ Proof. intros. simpl.
   rewrite Zpos_P_of_succ_nat. omega.
 Qed.
 
-Definition HTruePostCond t y x w nonce out c k h (xs:list int) ys Nonce C K OUT := 
+Definition HTruePostCond (FR:mpred) t y x w nonce out c k h (xs:list int) ys Nonce C K OUT := 
 (EX intsums:_,
   PROP (Zlength intsums = 16 /\
         (forall j, 0 <= j < 16 -> 
@@ -645,16 +620,15 @@ Definition HTruePostCond t y x w nonce out c k h (xs:list int) ys Nonce C K OUT 
    lvar _y (tarray tuint 16) y; lvar _x (tarray tuint 16) x;
    lvar _w (tarray tuint 16) w; temp _in nonce; temp _out out; temp _c c;
    temp _k k; temp _h (Vint (Int.repr h)))
-  SEP (SByte Nonce nonce; SByte C c;
+  SEP (FR; SByte Nonce nonce; SByte C c;
        ThirtyTwoByte K k;
        data_at Tsh (tarray tuint 16)
          (map Vint (hPosLoop2 4 intsums C Nonce)) x;
        data_at Tsh (tarray tuint 16) (map Vint ys) y;
-       data_at_ Tsh (tarray tuint 4) t; data_at_ Tsh (tarray tuint 16) w;
        data_at Tsh (tarray tuchar 64)
           (hPosLoop3 4 (hPosLoop2 4 intsums C Nonce) OUT) out)).
 
-Lemma verif_fcore_epilogue_htrue Espec t y x w nonce out c k h OUT xs ys Nonce C K:
+Lemma verif_fcore_epilogue_htrue Espec (FR:mpred) t y x w nonce out c k h OUT xs ys Nonce C K:
 @semax CompSpecs Espec
   (initialized_list [_i] (func_tycontext f_core SalsaVarSpecs SalsaFunSpecs))
   (PROP  ()
@@ -662,9 +636,8 @@ Lemma verif_fcore_epilogue_htrue Espec t y x w nonce out c k h OUT xs ys Nonce C
    lvar _y (tarray tuint 16) y; lvar _x (tarray tuint 16) x;
    lvar _w (tarray tuint 16) w; temp _in nonce; temp _out out; temp _c c;
    temp _k k; temp _h (Vint (Int.repr h)))
-   SEP  (data_at Tsh (tarray tuint 16) (map Vint xs) x;
+   SEP  (FR; data_at Tsh (tarray tuint 16) (map Vint xs) x;
    data_at Tsh (tarray tuint 16) (map Vint ys) y;
-   data_at_ Tsh (tarray tuint 4) t; data_at_ Tsh (tarray tuint 16) w;
    CoreInSEP (Nonce, C, K) (nonce, c, k); data_at Tsh (tarray tuchar 64) OUT out))
         (Ssequence
           (Ssequence
@@ -815,25 +788,32 @@ Lemma verif_fcore_epilogue_htrue Espec t y x w nonce out c k h OUT xs ys Nonce C
                 (Sset _i
                   (Ebinop Oadd (Etempvar _i tint)
                     (Econst_int (Int.repr 1) tint) tint))))))
-(normal_ret_assert (HTruePostCond t y x w nonce out c k h xs ys Nonce C K OUT)).
+(normal_ret_assert (HTruePostCond FR t y x w nonce out c k h xs ys Nonce C K OUT)).
 Proof. intros.
-forward_seq. apply HTrue_loop1; trivial.
+(*Lemma semax_nprmal_ret_assert_frame Espec Delta P L F R c RR: 
+      @semax CompSpecs Espec Delta (PROPx P (LOCALx L (SEPx R))) c
+                       (normal_ret_assert RR) -> 
+      @semax CompSpecs Espec Delta (PROPx P (LOCALx L (SEPx (F::R)))) c
+                       (normal_ret_assert (`F * RR)).*)
+freeze [0;3;4] FR1.
+forward_seq. apply HTrue_loop1. 
 Intros sums.
 destruct H as [SL [intsums [? HSums1]]]; subst sums. rewrite Zlength_map in SL.
-forward_seq.
 drop_LOCAL 0%nat.  
-apply (HTrue_loop2 Espec t y x w nonce out c k h OUT ys intsums Nonce C K); assumption.
+thaw FR1. freeze [0;2;4] FR2.
+forward_seq. apply HTrue_loop2.
 drop_LOCAL 0%nat.  
-eapply semax_post.
-  2: apply (HTrue_loop3 Espec t y x w nonce out c k h OUT 
-            (hPosLoop2 4 intsums C Nonce) ys Nonce C K); assumption.
-intros ? ?. apply andp_left2. unfold POSTCONDITION, abbreviate, HTruePostCond.
+thaw FR2. freeze [0;2;3;4;5] FR3.
+eapply semax_post. 2: apply HTrue_loop3.
+intros ? ?. apply andp_left2. unfold POSTCONDITION, abbreviate. (*, HTruePostCond.*)
 apply normal_ret_assert_derives'.
-Exists intsums. 
-Opaque ThirtyTwoByte. Opaque hPosLoop2. Opaque hPosLoop3.
-Time entailer!. (*6.6*)
-clear - HSums1 SL. intros j J.
+Exists intsums.
+clear - HSums1 SL.
+(*Opaque ThirtyTwoByte.*) Opaque hPosLoop2. Opaque hPosLoop3.
+Time entailer!. (*5.2 versus 6.6*)
+  intros j J.
   destruct (HSums1 _ J) as [xj [Xj [X _]]].
   destruct X as [yj [Yi Sj]]. apply J.
   exists xj, yj. auto.
-Time Qed. (*3*)
+thaw FR3. subst c k nonce. Time cancel. (*0.2 penalty*)
+Time Qed. (*3.8 versus 3 -- penalty*)
